f2effect: standardize naming
Ignore-this: b34c9e3dc5ce80a537337f7b90c37aee

darcs-hash:20131015082534-08f32-b897923c1aa8a9135e03821cc093a062368df72b

done/Iron/Language/SystemF2Effect/Step/FreshF.v
@@ -3,13 +3,46 @@ Require Export Iron.Language.SystemF2Effect.Step.Frame.
 
 
 (********************************************************************)
+(* Region identifier is not mentioned some FPriv frame. *)
+Fixpoint noprivF (p : nat) (f : frame) {struct f} :=
+ match f with
+ | FLet t x               => True
+ | FPriv None p1          => ~(p = p1)
+ | FPriv (Some p1) p2     => ~(p = p1) /\ ~(p = p2)
+ end.
+
+Definition noprivFs (p : nat) (fs : stack)
+ := Forall (noprivF p) fs.
+
+
+Lemma noprivFs_head 
+ :  forall p fs f
+ ,  noprivFs p (fs :> f)
+ -> noprivF  p f. 
+Proof.
+ intros. inverts H. eauto.
+Qed.
+Hint Resolve noprivFs_head.
+
+
+Lemma noprivFs_tail
+ :  forall p fs f
+ ,  noprivFs p (fs :> f)
+ -> noprivFs p fs. 
+Proof.
+ intros. inverts H. eauto.
+Qed.
+Hint Resolve noprivFs_tail.
+
+
+(********************************************************************)
 (* Region identifier is not mentioned in the given stack frame. *)
-Fixpoint freshF (p : nat) (ff : frame) {struct ff} 
- := match ff with
-    | FLet  t x           => freshT p t /\ freshX p x
-    | FPriv None      p2  => beq_nat p p2 = false
-    | FPriv (Some p1) p2  => beq_nat p p1 = false /\ beq_nat p p2 = false
-    end.
+Fixpoint freshF (p : nat) (ff : frame) {struct ff} :=
+ match ff with
+ | FLet  t x           => freshT p t /\ freshX p x
+ | FPriv None      p2  => beq_nat p p2 = false
+ | FPriv (Some p1) p2  => beq_nat p p1 = false /\ beq_nat p p2 = false
+ end.
 
 
 (* Region identifier is not mentioned in the given stack.  *)
@@ -18,38 +51,6 @@ Definition freshFs (p : nat) (fs : stack)
 Hint Unfold freshFs.
 
 
-(* Region identifier is not mentioned in the types of the free variables
-   of the given stack frame. *)
-Fixpoint   freshFreeF (p : nat) (te : tyenv) (f : frame) {struct f}
- := match f with
-    | FLet t x       => freshFreeX p (te :> t) x
-    | FPriv _ _      => True
-    end.
-
-
-(* Region identifier is not mentioned in the types of the free variables
-   of the given stack. *)
-Definition freshFreeFs (p : nat) (te : tyenv) (fs : stack)
- := Forall (freshFreeF p te) fs.
-Hint Unfold freshFreeFs.
-
-
-(* Region identifier is not mentioned in the types of the locations
-   used in the given stack frame. *)
-Fixpoint  freshSuppF   (p : nat) (se : stenv) (f : frame) {struct f}
- := match f with
-    | FLet  t x      => freshSuppX p se x
-    | FPriv _ _      => True
-    end.
-
-(* Region identifier is not mentioned in the types of the locations
-   used in the given stack. *)
-Definition freshSuppFs p2 se fs 
- := Forall (freshSuppF p2 se) fs.
-Hint Unfold freshSuppFs.
-
-
-(********************************************************************)
 Lemma freshFs_head 
  :  forall p f fs
  ,  freshFs p (fs :> f)
@@ -74,7 +75,47 @@ Proof. snorm. Qed.
 Hint Resolve freshFs_cons.
 
 
-(********************************************************************)
+Lemma freshF_noprivF
+ : forall p f
+ , freshF p f -> noprivF p f.
+Proof.
+ intros.
+ destruct f.
+ - snorm.
+ - destruct o; snorm.
+Qed.
+Hint Resolve freshF_noprivF. 
+
+
+Lemma freshFs_noprivFs
+ : forall  p fs
+ , freshFs p fs -> noprivFs p fs.
+Proof.
+ intros.
+ induction fs.
+ - unfold noprivFs. eauto.
+ - unfold noprivFs. inverts H. firstorder.
+Qed.
+Hint Resolve freshFs_noprivFs.
+
+
+(*********************************************************************)
+(* Region identifier is not mentioned in the types of the free variables
+   of the given stack frame. *)
+Fixpoint   freshFreeF (p : nat) (te : tyenv) (f : frame) {struct f} :=
+ match f with
+ | FLet t x       => freshFreeX p (te :> t) x
+ | FPriv _ _      => True
+ end.
+
+
+(* Region identifier is not mentioned in the types of the free variables
+   of the given stack. *)
+Definition freshFreeFs (p : nat) (te : tyenv) (fs : stack)
+ := Forall (freshFreeF p te) fs.
+Hint Unfold freshFreeFs.
+
+
 Lemma freshFreeF_nil
  :  forall p f
  ,  freshF p f
@@ -110,6 +151,22 @@ Hint Resolve freshFreeFs_tail.
 
 
 (********************************************************************)
+(* Region identifier is not mentioned in the types of the locations
+   used in the given stack frame. *)
+Fixpoint  freshSuppF   (p : nat) (se : stenv) (f : frame) {struct f} :=
+ match f with
+ | FLet  t x      => freshSuppX p se x
+ | FPriv _ _      => True
+ end.
+
+
+(* Region identifier is not mentioned in the types of the locations
+   used in the given stack. *)
+Definition freshSuppFs p2 se fs 
+ := Forall (freshSuppF p2 se) fs.
+Hint Unfold freshSuppFs.
+
+
 Lemma freshSuppFs_tail
  :  forall p te fs f
  ,  freshSuppFs p te (fs :> f)
@@ -130,4 +187,34 @@ Proof.
  inverts H. auto.
 Qed.
 Hint Resolve freshSuppFs_head.
+
+
+Lemma freshSuppF_mergeTE
+ :  forall p1 p2 p3 te f
+ ,  freshSuppF p1 te f
+ -> freshSuppF p2 te f
+ -> freshSuppF p2 (mergeTE p3 p1 te) f.
+Proof.
+ intros.
+ destruct f.
+ - snorm.
+   eapply freshSuppX_mergeTE; auto.
+ - eauto. 
+Qed.
+
+
+Lemma freshSuppFs_mergeTE
+ :  forall p1 p2 p3 te fs
+ ,  freshSuppFs p1 te fs
+ -> freshSuppFs p2 te fs
+ -> freshSuppFs p2 (mergeTE p3 p1 te) fs.
+Proof.
+ intros.
+ unfold freshSuppFs in *.
+ induction fs; auto.
+ inverts H.
+ inverts H0. rip.
+ eapply Forall_cons; auto.
+ eapply freshSuppF_mergeTE; auto.
+Qed.
 
