done/Iron/Language/SystemF2Effect/Store/Bind.v
@@ -3,7 +3,7 @@ Require Export Iron.Language.SystemF2Effect.Value.
 Require Export Iron.Language.SystemF2Effect.Value.Relation.TyJudge.WeakStProps.
 Require Export Iron.Language.SystemF2Effect.Value.Relation.TyJudge.TypeKind.
 
-
+(********************************************************************)
 (* Store bindings are the primitive objects we keep in the store.
    Each one is tagged with the number of the region is in. *)
 Inductive stbind :=
@@ -19,46 +19,49 @@ Hint Constructors stbind.
 Definition store := list stbind.
 
 
+(* Check whether some store binding is a live value. *)
 Definition isStValue (b : stbind)
  := exists p v, b = StValue p v.
 Hint Unfold isStValue.
 
 
+(* Check whether some store binding is dead *)
 Definition isStDead (b : stbind)
  := exists p,   b = StDead p.
 Hint Unfold isStDead.
 
 
-Definition regionOfStBind (b : stbind)
- := match b with 
-    | StValue p _ => p
-    | StDead  p   => p
-    end.
+(* Get the region identifier from a store binding. *)
+Definition regionOfStBind (b : stbind) := 
+ match b with
+ | StValue p _ => p
+ | StDead  p   => p
+ end.
 Hint Unfold regionOfStBind.
 
 
 (* Deallocate all store bindings in the given region by setting
    them to StDead. The dead bindings hold their locations in the
    store, but they no longer contain any value. *)
-Fixpoint deallocate (p1 : nat) (b : stbind) {struct b} : stbind
- := match b with
-    |  StValue p2 v
-    => if beq_nat p1 p2
-          then StDead  p2
-          else StValue p2 v
+Fixpoint deallocRegion (p1 : nat) (b : stbind) {struct b} : stbind := 
+ match b with
+ |  StValue p2 v
+ => if beq_nat p1 p2 then StDead  p2 else StValue p2 v
 
-    |  StDead p2
-    => StDead p2 
-    end.
+ | StDead p2
+ => StDead p2 
+ end.
 
 
-Fixpoint mergeB (p1 p2 : nat) (b : stbind) {struct b} : stbind
- := match b with
-    | StValue p v => StValue (if beq_nat p p2 then p1 else p) (mergeV p1 p2 v)
-    | StDead  p   => StDead  (if beq_nat p p2 then p1 else p)
-    end.
+(* Merge a store bind from the second region into the first. *)
+Fixpoint mergeB (p1 p2 : nat) (b : stbind) {struct b} : stbind := 
+ match b with
+ | StValue p v => StValue (if beq_nat p p2 then p1 else p) (mergeV p1 p2 v)
+ | StDead  p   => StDead  (if beq_nat p p2 then p1 else p)
+ end.
 
 
+(* Merge all store bindings in the second region into the first. *)
 Definition mergeBs p1 p2 bs
  := map (mergeB p1 p2) bs.
 
@@ -82,5 +85,4 @@ Proof.
  unfold isStDead. eauto.
 Qed.
 Hint Resolve isStDead_stdead.
-
 
