done/Iron/Language/SystemF2Effect/Store/StoreT.v
@@ -2,7 +2,7 @@
 Require Export Iron.Language.SystemF2Effect.Store.Bind.
 Require Export Iron.Language.SystemF2Effect.Store.TypeB.
 
-
+(********************************************************************)
 (* Well typed store.
    All bindings are well typed. *)
 Definition STORET' (sec : stenv) (se: stenv) (sp: stprops) (ss: store)
@@ -14,6 +14,7 @@ Definition STORET  (se  : stenv) (sp : stprops) (ss : store)
 Hint Unfold STORET.
 
 
+(********************************************************************)
 Lemma storeT_mergeB
  :  forall  sec se sp ss p1 p2
  ,  In (SRegion p1) sp
@@ -32,7 +33,7 @@ Qed.
 
 
 (* Weaken store properties in store typing judgement. *)
-Lemma storet_weak_stprops
+Lemma storeT_weak_stprops
  :  forall se sp ss p
  ,  STORET se sp ss
  -> STORET se (SRegion p <: sp) ss.
@@ -40,15 +41,15 @@ Proof.
  intros.
  unfold STORET in *.
  eapply Forall2_impl.
- - intros. eapply typeb_stprops_snoc. eauto.
+ - intros. eapply typeB_stprops_snoc. eauto.
  - auto.
 Qed.
-Hint Resolve storet_weak_stprops.
+Hint Resolve storeT_weak_stprops.
 
 
 (* All region handles in store bindings are present 
    in the store properties. *)
-Lemma storet_handles_in_stprops
+Lemma storeT_handles_in_stprops
  :  forall se sp ss
  ,  STORET se sp ss
  -> Forall (fun s => forall p
@@ -71,7 +72,7 @@ Qed.
 
 
 (* Extended store is well typed under extended store environment *)
-Lemma storet_snoc
+Lemma storeT_snoc
  :  forall se sp ss r1 v1 t2
  ,  KindT  nil sp (TRgn r1) KRegion
  -> TYPEV  nil nil se sp v1 t2
@@ -93,21 +94,19 @@ Proof.
       apply (typex_kind_type nil nil se sp (XVal v1) t2 (TBot KEffect)).
        auto. auto. auto.
  }
-     
+
  assert (Forall2 (TYPEB nil nil (tRef' <: se) sp) ss se).
  { lets D: (@Forall2_impl stbind ty) 
                 (TYPEB nil nil se sp) 
                 (TYPEB nil nil (tRef' <: se) sp)
                 ss se H1.
    intros.
-   apply typeb_stenv_snoc.
-    auto.
-    subst tRef'. eauto.
-   auto. 
+   apply typeB_stenv_snoc. auto. subst tRef'. eauto.
+   auto.
  }
 
  unfold STORET.
  auto.
 Qed.
-Hint Resolve storet_snoc.
+Hint Resolve storeT_snoc.
 
